src/Utils.dfy
@@ -6,11 +6,13 @@ module Utils {
     // what's polymorphism, precious?
 
     function method MinUInt64(a: uint64, b: uint64): uint64
+        ensures MaxUInt64(a, b) == a || MaxUInt64(a, b) == b
     {
         if a < b then a else b
     }
 
     function method MaxUInt64(a: uint64, b: uint64): uint64
+        ensures MaxUInt64(a, b) == a || MaxUInt64(a, b) == b
     {
         if a > b then a else b
     }
